src/Parsers/Reflective/ParserSemanticsOptimized.v
@@ -13,7 +13,7 @@ Module opt.
   Definition interp_has_parse_term
              (is_valid_nonterminal : list nat -> nat -> bool)
              (strlen : nat)
-             (char_at_matches : nat -> (Ascii.ascii -> bool) -> bool)
+             (char_at_matches_interp : nat -> Reflective.RCharExpr Ascii.ascii -> bool)
              (split_string_for_production : nat * (nat * nat) -> nat -> nat -> list nat)
              (t : has_parse_term interp_TypeCode) : bool
     := Eval cbv [step_option_rec] in
@@ -35,7 +35,7 @@ Module opt.
                      (fun parse_nt
                       => opt.interp_Term
                            f
-                           (fun n => char_at_matches n (*str*))
+                           (fun n => char_at_matches_interp n (*str*))
                            (fun n => split_string_for_production n (*str*))
                            len0 valid_len parse_nt valids offset len nt)
                      false
