src/Parsers/Reflective/ParserSoundness.v
@@ -13,11 +13,10 @@ Set Implicit Arguments.
 Section polypnormalize.
   Context (is_valid_nonterminal : list nat -> nat -> bool)
           (strlen : nat)
-          (char_at_matches : nat -> (Ascii.ascii -> bool) -> bool)
-          (split_string_for_production : nat * (nat * nat) -> nat -> nat -> list nat)
-          (char_at_matches_Proper : Proper (eq ==> pointwise_relation _ eq ==> eq) char_at_matches).
+          (char_at_matches_interp : nat -> Reflective.RCharExpr Ascii.ascii -> bool)
+          (split_string_for_production : nat * (nat * nat) -> nat -> nat -> list nat).
 
-  Let interp := interp_has_parse_term is_valid_nonterminal strlen char_at_matches split_string_for_production.
+  Let interp := interp_has_parse_term is_valid_nonterminal strlen char_at_matches_interp split_string_for_production.
 
   Lemma polypnormalize_correct (term : polyhas_parse_term)
     : ParserSyntaxEquivalence.has_parse_term_equiv
