src/Parsers/Reflective/ParserSyntax.v
@@ -1,8 +1,8 @@
 Require Import Fiat.Parsers.Reflective.Syntax.
 
 Local Notation rcStepT cbool :=
-  ((*Rchar_at_matches*)
-    (cnat --> (cascii --> cbool) --> cbool)
+  ((*Rchar_at_matches_interp*)
+    (cnat --> crchar_expr_ascii --> cbool)
       --> (*Rsplit_string_for_production*)
       (cnat * (cnat * cnat) --> cnat --> cnat --> (clist cnat))
       --> cnat --> cnat --> (cnat --> cnat --> cnat --> cbool) --> clist cnat --> cnat --> cnat --> cnat --> cbool)%typecode
